YLM: implemented third protocol step and event pred for first two steps
The aead pred and event pred for the third step still have to be defined

yahalom/YLM.Protocol.fst
@@ -111,3 +111,110 @@ let responder_send_msg_2 b kbs_idx msg1_idx =
     else error "[r_send_m2] actual initiator does not match with initiator in first message"
   )
   | _ -> error "[r_send_m2] wrong message"
+
+let find_auth_server_session (srv:principal) (p:principal) :
+  LCrypto (si:nat & vi:nat & st:session_st) (pki ylm_preds)
+  (requires (fun t0 -> True))
+  (ensures (fun t0 (|si,vi,st|) t1 -> trace_len t1 == trace_len t0 /\
+    valid_session (trace_len t0) srv si vi st /\
+    (match st with | AuthServerSession p' _ -> p = p' | _ -> False))) =
+  let now = global_timestamp () in
+  let filter = (fun si vi ser_st ->
+    match parse_session_st ser_st with
+    | Success (AuthServerSession p' _) -> p = p' | _ -> false) in
+
+  match find_session #ylm_preds #now srv filter with
+  | Some (|si,vi,ser_st|) ->
+    let Success st = parse_session_st ser_st in
+    (|si,vi,st|)
+  | None -> error ("[find_auth_server_session] no auth server session for " ^ p ^ " found")
+
+#push-options "--z3rlimit 100"
+let server_send_msg_3 srv msg2_idx =
+  // receive and parse second message
+  let (|now,b,ser_msg2|) = receive_i #ylm_preds msg2_idx srv in
+
+  match parse_msg ser_msg2 with
+  | Success (Msg2 b' c_ev_b) -> (
+    if b = b' then
+      // look up long term key with responder
+      let (|_,_,(AuthServerSession _ k_bs)|) = find_auth_server_session srv b in
+
+      // decrypt part of second message encrypted by responder
+      let iv = string_to_bytes #ylm_global_usage #now "iv" in
+      let ad = string_to_bytes #ylm_global_usage #now "ev2" in
+      match aead_dec #ylm_global_usage #now #(get_label ylm_key_usages k_bs) k_bs iv c_ev_b ad with
+      | Success ser_ev_b -> (
+        match parse_encval ser_ev_b with
+        | Success (EncMsg2 a n_a n_b) -> (
+          // look up long term key with initiator
+          let (|_,_,(AuthServerSession _ k_as)|) = find_auth_server_session srv a in
+
+          // generate communication key for initiator and responder
+          let (|_,k_ab|) = rand_gen #ylm_preds (readers [P srv; P a; P b]) (aead_usage "YLM.comm_key") in
+
+          // trigger event 'send key'
+          let prev = now in
+          let event = event_send_key a b srv n_a n_b k_ab in
+          trigger_event #ylm_preds srv event;
+
+          // create and send third message
+          let ev3_i = EncMsg3_I b k_ab n_a n_b in
+          let now = global_timestamp () in
+          assert(is_publishable ylm_global_usage prev k_bs \/ aead_pred ylm_usage_preds prev "YLM.lt_key" k_bs ser_ev_b ad);
+          aead_dec_plaintext_publishable_if_key_and_ciphertext_publishable_forall ylm_global_usage;
+          assert(is_publishable ylm_global_usage prev ser_ev_b \/ aead_pred ylm_usage_preds prev "YLM.lt_key" k_bs ser_ev_b ad);
+          splittable_term_publishable_implies_components_publishable_forall ylm_global_usage;
+          assert(is_publishable ylm_global_usage prev n_a /\ is_publishable ylm_global_usage prev n_b
+            \/ aead_pred ylm_usage_preds prev "YLM.lt_key" k_bs ser_ev_b ad);
+          readers_is_injective_2 b srv;
+          assert(is_publishable ylm_global_usage prev n_a /\ is_publishable ylm_global_usage prev n_b
+            \/ did_event_occur_before prev b (event_req_key a b srv n_a n_b));
+          assert(is_publishable ylm_global_usage prev n_a /\ is_publishable ylm_global_usage prev n_b
+            \/ (exists i. i < prev /\ is_msg ylm_global_usage i n_a public
+            /\ was_rand_generated_before i n_b (readers [P b; P a; P srv]) (nonce_usage "YLM.nonce_b")));
+          can_flow_later_forall cpred (get_label ylm_key_usages n_a) public;
+          rand_is_secret #ylm_global_usage #now #(readers [P b; P a; P srv]) #(nonce_usage "YLM.nonce_b") n_b;
+          assert(is_publishable ylm_global_usage now n_a /\ is_publishable ylm_global_usage now n_b
+            \/ (exists i. later_than now i /\ is_valid ylm_global_usage i n_a /\ can_flow i (get_label ylm_key_usages n_a) public)
+            /\ is_secret ylm_global_usage now n_b (readers [P b; P a; P srv]) (nonce_usage "YLM.nonce_b"));
+          assert(is_msg ylm_global_usage now n_a public /\ is_publishable ylm_global_usage now n_b \/ is_secret ylm_global_usage now n_b (readers [P b; P a; P srv]) (nonce_usage "YLM.nonce_b"));
+          flows_to_public_can_flow now (get_label ylm_key_usages n_a) (get_label ylm_key_usages k_as);
+          flows_to_public_can_flow now (get_label ylm_key_usages n_b) (get_label ylm_key_usages k_as);
+          includes_can_flow_lemma now [P b; P a; P srv] [P a; P srv];
+          assert(is_msg ylm_global_usage now n_a (get_label ylm_key_usages k_as));
+          assert(is_msg ylm_global_usage now n_b (get_label ylm_key_usages k_as));
+          let ser_ev3_i = serialize_encval now ev3_i (get_label ylm_key_usages k_as) in
+          let ad = string_to_bytes #ylm_global_usage #now "ev3_i" in
+          parse_serialize_encval_lemma now ev3_i (get_label ylm_key_usages k_as);
+          let c_ev3_i = aead_enc #ylm_global_usage #now #(get_label ylm_key_usages k_as) k_as iv ser_ev3_i ad in
+
+          let ev3_r = EncMsg3_R a k_ab in
+          includes_can_flow_lemma now [P srv; P a; P b] [P b; P srv];
+          let ser_ev3_r = serialize_encval now ev3_r (get_label ylm_key_usages k_bs) in
+          let ad = string_to_bytes #ylm_global_usage #now "ev3_r" in
+          parse_serialize_encval_lemma now ev3_r (get_label ylm_key_usages k_bs);
+          let c_ev3_r = aead_enc #ylm_global_usage #now #(get_label ylm_key_usages k_bs) k_bs iv ser_ev3_r ad in
+
+          let msg3 = Msg3 c_ev3_i c_ev3_r in
+          let ser_msg3 = serialize_msg now msg3 in
+
+          let msg3_idx = send #ylm_preds #now srv a ser_msg3 in
+
+          // store server session
+          let new_sess_idx = new_session_number #ylm_preds srv in
+          let st_srv_sent_m3 = AuthServerSentMsg3 a b k_ab in
+          let now = global_timestamp () in
+          let ser_st = serialize_session_st now srv new_sess_idx 0 st_srv_sent_m3 in
+
+          new_session #ylm_preds #now srv new_sess_idx 0 ser_st;
+
+          (msg3_idx, new_sess_idx)
+        )
+        | _ -> error "[srv_send_m3] wrong responder encval"
+      )
+      | Error e -> error ("[srv_send_m3] " ^ e)
+    else error "[srv_send_m3] actual responder does not match with responder in second message"
+  )
+  | _ -> error "[srv_send_m3] wrong message"
+#pop-options
