yahalom/YLM.Helper.fst
@@ -1,0 +1,7 @@
+module YLM.Helper
+
+
+friend CryptoLib
+
+
+let split_is_split_len_prefixed b = ()
