yahalom/YLM.Helper.fsti
@@ -1,0 +1,9 @@
+module YLM.Helper
+
+
+open CryptoLib
+
+
+val split_is_split_len_prefixed: b:bytes ->
+  Lemma (split b == split_len_prefixed 4 b)
+        [SMTPat (split b)]
